Big commit for CSE
- Remove Tuple (not everywhere, because of some eval_type)
- Stop sharing reads (because of dependent types) (makes Isa with 128 bindings instead of 101)
- Minor trouble for sval_eqb_correct (but nothing complicated remains)

src/CSE.v
@@ -18,7 +18,7 @@ Section t.
 
   Inductive sval : type -> Type :=
   | SVar: forall t, nat -> sval t
-  | SRead : forall t, Common.var Phi (Treg t) -> sval t
+  (* | SRead : forall t, Common.var Phi (Treg t) -> sval t *)
   | SConstant : forall t, constant t -> sval t
   | SMux : forall t, sval Tbool -> sval t -> sval t -> sval t
   | STuple : forall l, DList.T sval l ->  sval (Ttuple l)
@@ -26,10 +26,56 @@ Section t.
                  DList.T sval arg -> 
                  sval res. 
 
+    
+  Section induction. 
+    (** Since the induction principle that is generated is not
+      useful, we have to define our own.  *)
+    
+      Variable P : forall t : type, sval t -> Prop.  
+      Hypothesis Hvar : forall (t : type) (v : nat), P t (SVar t v). 
+      Hypothesis Hconstant : 
+      forall (ty : type) (c : constant ty), P ty (SConstant ty c). 
+      Hypothesis Hmux : forall (t : type) (e : sval B) (l r : sval t),
+                          P B e -> P t l -> P t r ->  P t (SMux t e l r ).  
+      Hypothesis Htuple : forall (l : list type) (exprs : DList.T sval l),
+                            DList.Forall _ _ P l exprs -> 
+                            P (Ttuple l) (STuple l exprs). 
+      Hypothesis Hbuiltin : 
+      forall (args : list type) (res : type) (f0 : builtin args res)
+        (t : DList.T sval args), 
+        DList.Forall _ _ P args t ->
+        P res (SBuiltin args res f0 t). 
+
+      Lemma sval_ind_alt (t : type) (sv : sval t) :  P t sv. 
+      refine (let fix fold (t : type) (sv : sval t) :  P t sv  := 
+                  match sv with
+                    | SVar t x => Hvar t x
+                    | SConstant t x => Hconstant t x
+                    | SMux t x x0 x1 => Hmux t _ _ _ (fold _ x) (fold _ x0) (fold _ x1)
+                    | STuple l x => Htuple l x _ 
+                    | SBuiltin arg res f x => Hbuiltin arg res f _ _
+                  end in fold t sv). 
+      {
+        induction x. simpl; apply I.
+        split; [apply fold | apply IHx]; auto.      
+      }
+      { clear f. 
+        induction x. simpl; apply I. 
+        split; [apply fold | apply IHx]; auto. }
+      Qed. 
+  End induction. 
+
+
   Arguments STuple {l}%list _%dlist. 
   Arguments SBuiltin {arg res} f _%dlist. 
-  
-  Definition eval_sval t ( sv : sval t) (env : forall t, list (eval_type t) )  : option (eval_type t).
+
+  Definition type_cast {P : type -> Type} {t} t' (x : P t) : option (P t'). 
+  case_eq (type_eqb t t'). 
+  intros. apply (type_eqb_correct t t') in H. subst. apply Some. auto. 
+  intros. apply None. 
+  Defined.
+
+  Definition eval_sval t ( sv : sval t) (env : list ({t : type & eval_type t}) )  : option (eval_type t).
   refine (let fix eval_sval t (sv : sval t) : option (eval_type t) := 
               let fold :=
                   (fix fold l dl  : option (eval_type (Ttuple l)):=
@@ -42,8 +88,14 @@ Section t.
                    end%dlist)
               in
                 match sv with              
-                  | SVar t n => List.nth_error (env t) n
-                  | SRead t v => Some (Common.Tuple.get _ _ v st)
+                  | SVar t n => 
+                      do tx <- List.nth_error (env) n;
+                      match tx with 
+                          existT t' x => 
+                            type_cast t x
+                      end 
+                            
+                  (* | SRead t v => Some (Common.DList.get v st) *)
                   | SConstant t x => Some x
                   | SMux t c l r  => 
                       do c <- eval_sval _ c;
@@ -53,17 +105,9 @@ Section t.
                 | STuple l x => 
                     fold _ x
                 | SBuiltin arg res f x => 
-                    do x <- _;
+                    do x <- fold _ x;
                     Some (builtin_denotation _ _ f x)
               end in eval_sval t sv).
-  refine ((fix fold l (dl : DList.T _ l): option (eval_type_list l) :=
-          match dl in DList.T _ l' return (option (eval_type_list l')) with 
-                                       | [] => Some tt
-                                       | t :: q => 
-                                           do t <- eval_sval _ t;
-                                           do q <- fold _ q;
-                                           Some ((t,q))
-          end%dlist) _ x). 
   Defined. 
 
 
@@ -86,26 +130,27 @@ Section t.
   Definition cse_expr t (e : expr Phi V t) : expr Phi Var t * option (sval t). 
   refine (
       match e  with
-        | Eread t v => (Eread _ _ t v, Some (SRead t v))
+        (* | Eread t v => (Eread _ _ t v, Some (SRead t v))  *)
+        | Eread t v => (Eread _ _ t v, !!)
         | Eread_rf n t v adr =>   (Eread_rf _ _ _  t v (fst adr), !! )
         | Ebuiltin args res f x => let v := DList.map (fun x dx => fst dx) x in 
-                                   let sv  := DList.map (fun x dx => snd dx) x in                                    (Ebuiltin _ _ args res f v ,  Some (SBuiltin f sv) )
-        | Econstant ty c => (Econstant _ _ _ c, Some (SConstant _ c))
-        | Emux t c l r =>  (Emux _ _ _ (fst c) (fst l) (fst r), !!) 
+                                    let sv  := DList.map (fun x dx => snd dx) x in                                     (Ebuiltin _ _ args res f v ,  Some (SBuiltin f sv) ) 
+        | Econstant ty c =>  (Econstant _ _ _ c, Some (SConstant _ c)) 
+        | Emux t c l r =>   (Emux _ _ _ (fst c) (fst l) (fst r), !!) 
         | Efst l t x => (Efst _ _ _ _ (fst x), 
                         match snd x in sval t' return fstT t' with
-                          | @STuple (_ :: _) dl => Some  (DList.hd _ _ _ _ dl)
+                          | @STuple (_ :: _) dl => Some  (DList.hd  dl)
                           | _ => !!
                         end)
         | Esnd l t x => (Esnd _ _ _ _ (fst x), 
                         match snd x in sval t' return sndT t' with
-                          | @STuple (t::q) dl => Some  (@STuple q (DList.tl _ _ _ _ dl))
+                          | @STuple (t::q) dl => Some  (@STuple q (DList.tl  dl))
                           | _ => !!
                         end)
         | Enth l t m x => (Enth _ _ _ _ m (fst x), 
                           match snd x in sval t' return nthT  t' t 
                           with
-                            | @STuple l dl => fun m => Some (DList.get _ _ _ _ m dl)
+                            | @STuple l dl => fun m => Some (DList.get  m dl)
                             | _ => fun _ => !!
                           end m) 
         | Etuple l exprs => let x := DList.map (fun x dx => fst dx) exprs in 
@@ -125,7 +170,7 @@ Section t.
                   end%dlist in 
 
               match va, vb with
-                | SRead ta va, SRead tb vb => var_eqb va vb 
+                (* | SRead ta va, SRead tb vb => var_eqb va vb  *)
                 | SVar ta na, SVar tb nb  => type_eqb ta tb && NPeano.Nat.eqb na nb
                 | SConstant ta ca, SConstant tb cb =>
                     _
@@ -142,34 +187,29 @@ Section t.
   exact (fun _ => false). 
   Defined. 
   
-  Record Env := mk
-    {
-      content : forall t : type , list (sval t * Var t);
-      next : nat              
-    }. 
+  Definition Env := list ({t : type & (sval t * Var t)%type}). 
 
-  Definition empty : Env := mk (fun _ => [])%list 0. 
+  Definition empty : Env := ([])%list. 
 
-  Definition lookup (t : type) (sv: sval t) (E : Env) : option (Var t).
-  refine (let l := content E t in 
-            let fix lookup sv l :=
-                match l with 
-                  | [] => None
-                | (sv',x) :: b => if sval_eqb _ _ sv sv' then Some x else lookup sv b
-                end%list in 
-              lookup sv l                 
-         ). 
-  Defined.
+  Fixpoint lookup (t : type) (sv: sval t) (E : Env) : option (Var t) :=
+    match E with 
+      | [] => None
+      | existT  t' (sv',x)::q => 
+          (if type_eqb t' t as b 
+              return type_eqb t' t = b -> option (Var t)
+           then
+             (fun H : type_eqb t' t = true  => 
+                let H := type_eqb_correct t' t H in 
+                  if sval_eqb _ _ sv sv' 
+                  then Some (eq_rect t' Var x t H)
+                  else lookup _ sv q                                 
+             )
+              else 
+            fun _ => lookup t sv q) eq_refl
+    end%list. 
 
-  Definition add (t : type) (sv : sval t) (v : Var t) : Env -> Env. 
-  intros E.  
-  refine (mk _ _ ). 
-  intros t'. 
-  case_eq (type_eqb t t'). 
-  intros. apply type_eqb_correct in H. subst. apply ((sv,v) :: content E t')%list.  
-  intros _. apply (content E t'). 
-  apply (S (next E)). 
-  Defined. 
+  Definition add (t : type) (sv : sval t) (v : Var t) (env : Env) : Env :=
+    ( env ++ [existT _ t (sv,v)])%list . 
 
   (* Unfortunately, multiple reads from the same state elements cannot be shared *)
   Definition cse_telescope {A} (E: Env) (T : telescope Phi V A) : telescope Phi Var A. 
@@ -181,7 +221,7 @@ Section t.
   refine (let (e,svo) := cse_expr arg b in _). 
   refine (match svo with 
               | None => k :- e; 
-                  let sv := (SVar arg (next F)) in
+                  let sv := (SVar arg (List.length F)) in
                     let F := add arg  sv k F in
                       cse F (cont (k,sv))
               | Some sv =>                   
@@ -197,7 +237,7 @@ Section t.
 
 
   Definition cse_effects (eff: effects Phi V) : effects Phi Var. 
-  refine( Tuple.map _ Phi eff). 
+  refine( DList.map  _  eff). 
   intros a x. 
   refine (match x with 
             | None => None
@@ -219,84 +259,492 @@ End t.
 
 Import Flat. 
 
-Notation V := (fun t => (eval_type t * sval _ t))%type.  
-Definition lift {Phi} : Env Phi eval_type -> (forall t, list (eval_type t)). 
-intros. 
-apply (List.map (@snd _ _) (content _ _ X t)). 
-Defined. 
+Notation V := (fun t => (eval_type t * sval t))%type.  
 
-Ltac t :=   repeat match goal with 
-                       H : existT _ _ _ = existT _ _ _ |- _ => apply Eqdep.EqdepTheory.inj_pair2 in H
-                   end.
-Notation "G |- x -- y" := (In _ _ _ x y G) (no associativity, at level 71). 
+Require Import Eqdep. 
+
+
+Ltac t :=  subst; repeat match goal with 
+                       H : existT _ _ _ = existT _ _ _ |- _ => 
+                         apply Eqdep.EqdepTheory.inj_pair2 in H
+                   |   H : context [eq_rect ?t _ ?x ?t ?eq_refl] |- _ => 
+                         rewrite <- eq_rect_eq in H
+                   |   H : context [eq_rect ?t _ ?x ?t ?H'] |- _ => 
+                         rewrite (UIP_refl _ _ H') in H;
+                         rewrite <- eq_rect_eq in H
+                   |   H : existT _ ?t1 ?x1 = existT _ ?t2 ?x2 |- _ => 
+                         let H' := fresh "H'" in 
+                           apply eq_sigT_sig_eq in H; destruct H as [H H']; subst
+                         end; subst.
+
+
+Ltac d :=
+  match goal with 
+   H : context [do _ <- ?x; _] |- _ =>
+     let A := fresh in 
+     case_eq x; [intros ?X A | intros A]; rewrite A in H; simpl in H
+  | |- context [do _ <- ?x; _] =>
+     case_eq x; intros; simpl
+  end.
+Ltac f := 
+  match goal with 
+      |- context [fst ( _ , _ )] => simpl
+    | |- context [fst ?x] => destruct x; simpl
+    | |- context [Tuple.fst ( _ , _ )] => simpl
+    | |- context [Tuple.fst ?x] => destruct x; simpl
+    | |- context [snd ( _ , _ )] => simpl
+    | |- context [snd ?x] => destruct x; simpl
+    | |- context [Tuple.snd ( _ , _ )] => simpl
+    | |- context [Tuple.snd ?x] => destruct x; simpl
+  end;
+  try (congruence || discriminate). 
+Notation "G |= x -- y" := (In _ _ _ x y G) (no associativity, at level 71). 
 
 Notation R := (fun G t x y => In _ _ t x y G).  
 
-Require Import Equality. 
-Lemma cse_expr_correct Phi st : forall t e1 r1, 
+Definition lift (env : Env eval_type) : list ({t : type & eval_type t}). 
+refine (List.map _ env). 
+refine (fun x => match x with  existT t (sv,v) => existT _ t v end). 
+Defined. 
+
+Record Gamma_inv (G : Gamma eval_type V) (E : Env eval_type) :=
+  {
+    Gamma_inv_1 : forall t (x : eval_type t) y, G |= x -- y -> x = fst y;
+    Gamma_inv_2 : forall t x y, G |= x -- y -> eval_sval t (snd y) (lift E) = Some x;
+    Gamma_inv_3 : forall t x sv, List.In (existT _ t (sv , x))  E -> G |= x -- (x,sv)
+  }. 
+ 
+Hint Resolve Gamma_inv_1 Gamma_inv_2 Gamma_inv_3. 
+
+Ltac use :=
+  match goal with 
+    | Hgamma : Gamma_inv ?G _,  H : ?G |= ?x -- ?y |- context [?x] =>
+        rewrite (Gamma_inv_1 _ _  Hgamma _ _ _ H) 
+  end. 
+
+
+Section test. 
+  Import Equality. 
+  Lemma cse_expr_correct Phi st : forall t e1 r1, 
   eval_expr Phi st t e1 = r1 ->
-  forall G (env : Env Phi eval_type) e2,
+  forall G (env : Env eval_type) e2,
     expr_equiv _ _ Phi (R G) t e1 e2 ->     
-    (forall t (x : eval_type t) y, G |- x -- y -> x = fst y)  ->
-    (forall t (x : eval_type t) y, G |- x -- y -> eval_sval Phi st t (snd y) (lift env) = Some x)
+    (forall t (x : eval_type t) y, G |= x -- y -> x = fst y)  ->
+    (forall t (x : eval_type t) y, G |= x -- y -> eval_sval t (snd y) ( lift env) = Some x)
     -> match snd (cse_expr Phi _ t  e2) with
-        | Some sv => eval_sval Phi st t sv (lift env) = Some r1
+        | Some sv => eval_sval  t sv ( lift env) = Some r1
         | None => True
       end.
 Proof. 
-  destruct 1; inversion 1; t; subst; try solve [simpl; auto].  
-  - admit. 
+  destruct 1; inversion 1; t;  try solve [simpl; auto].  
+  - intros. 
+    clear H. 
+    simpl. 
+    d. repeat f_equal. 
+    revert H. clear f. 
+    induction args. 
+    simpl; repeat DList.inversion.  simpl. congruence. 
+    simpl. repeat DList.inversion. simpl in *. repeat d. repeat f_equal.
+
+    apply DList.inversion_pointwise in H3. destruct H3.   
+    pose proof (H1 _ _ _ H5). destruct o. 
+    f_equal. congruence. 
+    apply (IHargs x2) in H4. 
+    congruence.  auto.
+
+    discriminate. 
+    discriminate. 
+    discriminate. 
+    simpl. 
+    
+    apply False_rect. 
+    clear f. 
+    
+    induction args. 
+    repeat DList.inversion. simpl in *. discriminate.
+    repeat DList.inversion. simpl in *. repeat d; try discriminate.
+    apply DList.inversion_pointwise in H3. eapply IHargs.
+    destruct H3. apply H3. apply H4.  
+    apply DList.inversion_pointwise in H3. 
+    destruct H3. apply H1 in H4. congruence. 
+
   - intros.  simpl. 
-    destruct dl2 as [hd tl].  simpl. dependent destruction tl; try tauto.    
-    erewrite <- H1. 
-    Focus 2.
+    destruct dl2 as [hd tl].  simpl. dependent destruction tl; try tauto.
+    specialize (H0 _ _ _ H3). 
+    specialize (H1 _ _ _ H3). 
+    DList.inversion; subst. simpl in *; repeat d; f. 
+  - t .  intros. 
+    specialize (H1 _ _ _ H2).
+    specialize (H3 _ _ _ H2).
+    simpl.     destruct dl2 as [hd tl].  simpl. dependent destruction tl; try tauto.
+    subst. simpl in *.   DList.inversion. subst. simpl. 
+    repeat d; f. 
+  - intros. simpl.  
+    destruct dl2 as [hd tl]. simpl.  dependent destruction tl; try tauto.
+    simpl. 
+    clear H.
+    specialize (H1 _ _ _ H3). clear H3. 
+    induction v. 
+    + simpl. simpl in H1. DList.inversion. subst.      
+      
+      repeat d; simpl; f.  
+    + simpl. 
+      erewrite IHv. reflexivity. 
+      simpl. 
+      DList.inversion. subst. simpl. simpl in H1. 
+      repeat d; simpl; f. 
+  - intros.  simpl. 
+    t.   clear H H0 H4. 
+    induction l. 
+
+    + simpl; repeat DList.inversion. 
+      simpl in *. 
+      reflexivity. 
+    + repeat DList.inversion. simpl in *. 
+    destruct (DList.inversion_pointwise _ _ _ _ _ _ _ H2). clear H2. 
     
-    simpl in dl1. simpl in hd.  destruct dl1. simpl. 
+    repeat d; subst.
+    * erewrite IHl in H4. clear IHl.  2: apply H. solve [firstorder congruence]. 
+    * erewrite IHl in H4. clear IHl.  2: apply H. congruence. 
+    * clear IHl.    firstorder congruence. 
     
-    Lemma inversion_dlist {A F} : forall (t : A) q (dl : DList.T F (t :: q)), 
-                                exists hd tl, dl = (hd :: tl)%dlist. 
-    Admitted. 
-    destruct (inversion_dlist _ _ t0) as [t01 [t02 H''] ]. subst. 
-    pose (H'' := H1 _ _ _ H3). clearbody H''. simpl in H''. 
-    repeat match goal with 
-        H : context [do _ <- ?x; _] |- _ => destruct x; simpl in H
-    end. 
-    injection H''. intros; subst. 
-Admitted. 
-(*
-    match goal with 
-        |- context [do _ <- ?x; _] => 
-          assert (x = Some (DList.to_tuple (fun x X => X) t))
-    end. 
-  clear H0. 
-  induction dl2.  simpl.
-  clear. assert (t = DList.nil). 
-  Require Import Equality. dependent destruction t. reflexivity. 
-  rewrite H. simpl. reflexivity. simpl. 
-  Ltac d := (match goal with 
-              |- context [do _ <- ?x; _] => case_eq x; intros; simpl
-          end). 
-  d. d.
-  f_equal. dependent destruction t. simpl.
-  f_equal. 
+    Grab Existential Variables. 
+    simpl in *. destruct dl1.  auto. 
+Qed. 
+End test. 
 
-  simpl. 
-  simpl. 
-  
 
-  inversion t. 
-  
-
-  
  
+Lemma lem1 Phi st env G  t e1 e2 e'  sv : 
+  expr_equiv eval_type V Phi (Flat.R eval_type V G) t e1 e2 ->
+  Gamma_inv G env ->
+  cse_expr Phi eval_type t e2 = (e', Some sv) ->
+  eval_sval t sv (lift env) = Some (eval_expr Phi st t e1). 
+Proof. 
+  intros H H1 H2.  
+  pose (H' := cse_expr_correct _ st _ _ (eval_expr Phi st t e1) (refl_equal)). 
+  specialize (H' G env e2 H). 
+  specialize (H' (Gamma_inv_1 _ _ H1) (Gamma_inv_2 _ _ H1)).
+  rewrite H2 in H'.
+  apply H'. 
+Qed.
+
+Lemma type_eqb_refl : forall t, type_eqb t t = true. 
+induction t using type_ind; simpl;  firstorder. 
+apply NPeano.Nat.eqb_eq. reflexivity. 
+apply NPeano.Nat.eqb_eq. reflexivity. 
+Qed. 
+ 
+Section protect00. 
+Import Equality. 
+Lemma sval_eqb_correct t (sv sv' : sval t) : sval_eqb t t sv sv' = true -> sv = sv'. 
+Proof. 
+  revert sv'. 
+  induction sv using sval_ind_alt; dependent destruction sv'; simpl;
+  intros;
+  repeat 
+    match goal with 
+        H: (?x && ?y)%bool = true |- _ => rewrite Bool.andb_true_iff in H; destruct H
+      | H : type_eqb _ _ = true |- _ => apply type_eqb_correct in H
+      | H : NPeano.Nat.eqb _ _ = true |- _ => apply NPeano.Nat.eqb_eq in H
+    end; subst; try discriminate; auto.
+  - revert H. 
+  generalize (type_eqb_refl t). 
+  generalize (type_eqb_correct t t). 
+  destruct (type_eqb t t); try discriminate.  
+  intros. unfold eq_rect_r in H0. rewrite (UIP_refl _ _ (e eq_refl)) in H0.
+  rewrite (UIP_refl _ _ (eq_sym eq_refl)) in H0. 
+  rewrite <- eq_rect_eq in H0. 
+  clear - H0. admit. 
+  - repeat match goal with 
+      | H : forall t, _ -> _ , H' : _ |- _ => apply H in H'; clear H; rewrite H'
+  end. reflexivity.
+  - induction l; repeat DList.inversion. reflexivity.   
+    simpl in *. rewrite Bool.andb_true_iff in H0. destruct H0.
+    repeat f_equal. 
+    destruct H. auto. 
+    destruct H. specialize (IHl _ H2 _ H1). clear - IHl. injection IHl; intros; t; auto. 
+Admitted. 
+
+End protect00. 
+
+Lemma lookup_1 env t (sv : sval t) e :
+  lookup eval_type t sv (env) = Some e ->
+  List.In (existT _ t (sv,e)) (env). 
+Proof.
+  intros. 
+  induction env. discriminate.
+  destruct a as [t' [sv' x']]. simpl in H.
+  revert H. generalize (type_eqb_correct t' t). destruct (type_eqb t' t).  simpl. intros.
+  pose proof (e0 eq_refl). subst. 
+
+  case_eq (sval_eqb t t sv sv'); intros.    
+  left. t. rewrite H0 in H. 
+  repeat f_equal; try congruence || symmetry; auto using sval_eqb_correct. 
+  right.  apply IHenv. rewrite H0 in H.  auto. 
+  intros. 
+  simpl. right. auto. 
+Qed. 
+
+Lemma lem2  G env t e1 e2 sv : 
+  List.In (existT _ t (sv,e2)) (env) ->
+  Gamma_inv G env ->
+  eval_sval t sv (lift env) = Some e1 ->
+  G |= e1 -- (e2, sv). 
+Proof. 
+  intros. apply (Gamma_inv_3 _ _ H0) in H. 
+  pose proof (Gamma_inv_2 _ _ H0 _ _ _ H). 
+  simpl in H2. 
+  
+  assert ( e1 = e2). congruence.
+  subst; auto. 
+Qed. 
+
+Lemma lemma_2 Phi st env G  t e1 e2 e3 e'  sv : 
+  expr_equiv eval_type V Phi (Flat.R eval_type V G) t e1 e2 ->
+  Gamma_inv G env ->
+  cse_expr Phi eval_type t e2 = (e', Some sv) ->
+  lookup eval_type t sv (env) = Some e3 ->
+  eval_expr Phi st t e1 = e3. 
+Proof. 
+  intros. 
+  assert (eval_sval t sv (lift env) = Some (eval_expr Phi st t e1)). eauto using lem1.
+  
+  apply lookup_1 in H2.   
+  apply (Gamma_inv_3 _ _ H0) in H2. 
+  apply (Gamma_inv_2 _ _ H0) in H2. 
+  simpl in H2. congruence. 
+Qed. 
+
+Lemma Gamma_inv_cons G env t e sv : 
+  Gamma_inv G env ->
+  eval_sval t sv (lift env)  = Some e ->
+  Gamma_inv (cons eval_type V t e (e,sv) G) env. 
+Proof. 
+  intros. constructor. 
+  - intros. inversion H1; t. reflexivity. eauto. 
+  - intros. inversion H1; t. simpl. eauto.  eauto. 
+  - intros. apply In_skip. eauto. 
+Qed. 
+
+Ltac clean := repeat match goal with H : ?x = ?x |- _ => clear H end. 
+
+Section protect. 
+Lemma cse_effects_correct Phi st Delta G e  (Hg : Gamma_inv G e):
+  forall e1 e2 
+  (H : effects_equiv eval_type V Phi (Flat.R eval_type V G) e1 e2), 
+   eval_effects Phi st e1 Delta =
+   eval_effects Phi st (cse_effects Phi eval_type e2) Delta. 
+Proof. 
+  intros e1 e2 H. induction H; subst; repeat t; subst. 
+  - simpl; reflexivity. 
+  - intros. 
+    clean. 
+    simpl. 
+    Import Equality.     
+    repeat match goal with 
+      |- context [match ?x with _ => _ end] => first [destruct x | dependent destruction x]
+    end; intros;
+    unfold eval_state in *; repeat DList.inversion; subst; simpl in *;
+    intros; inversion H; t; unfold Flat.R in *; simpl; repeat auto;
+    repeat match goal with 
+      |- (_ :: _ = _ :: _)%list => f_equal
+    | |- (_ :: _ = _ :: _)%dlist => f_equal
+    | |- _ => auto
+    end. 
+    destruct x; [reflexivity | repeat use; reflexivity]. 
+    destruct x; [reflexivity | repeat  use; reflexivity]. 
+Qed. 
+End protect. 
+
+Lemma type_cast_eq t (e : eval_type t) : type_cast t e = Some e. 
+Proof. 
+  unfold type_cast.
+  generalize (type_eqb_correct t t). intros. 
+  assert (H := type_eqb_refl). 
+  generalize (H t). 
+  destruct (type_eqb t t). 
+  
+  rewrite (UIP_refl _ _ (e0 eq_refl)).  
+  simpl. reflexivity. 
+  discriminate. 
+Qed. 
+
+Lemma nth_error_app {A} l :
+  forall l' n (x : A), List.nth_error l n = Some x ->
+                  List.nth_error (l ++ l') n = Some x. 
+Proof. 
+  induction l. simpl. destruct n; discriminate. 
+  simpl. intros. destruct n. simpl in *. auto. 
+  
+  simpl. auto. 
+Qed.
+
+Lemma eval_sval_monotone l l' t x : 
+  forall sv,  
+    eval_sval t sv l = Some x  ->
+    eval_sval t sv (l ++ l') = Some x. 
+Proof. 
+  induction sv using sval_ind_alt. simpl. 
+
+  d. simpl in H0.
+  rewrite (nth_error_app _ _ _ _ H). simpl. auto. 
+  simpl in *. discriminate. 
+  simpl. auto. 
+  simpl in *. 
+  intros.  invert_do H. 
+  
+  repeat match goal with 
+      | H : forall t, _ -> _ , H' : _ |- _ => apply H in H'; clear H; rewrite H'
+  end. reflexivity.
+  
+  induction exprs. simpl. auto.
+  intros H'.
+  simpl in H. destruct H as [Hhd Htl]. 
+  simpl. simpl in H'.  invert_do H'. apply Hhd in EQ. rewrite EQ. clear EQ. simpl. 
+  apply IHexprs in EQ1; auto. simpl in EQ1. rewrite EQ1. simpl. reflexivity. 
+  
+  simpl.  
+  assert (forall x, 
+      let dl := (fix fold (l0 : list type) (dl : DList.T (fun H0 : type => sval H0) l0)
+              {struct dl} : option (Tuple.of_list eval_type l0) :=
+       match
+         dl in (DList.T _ l1) return (option (Tuple.of_list eval_type l1))
+       with
+       | DList.nil => Some tt
+       | DList.cons t0 q0 t1 q =>
+           do t2 <- eval_sval t0 t1 l; do q1 <- fold q0 q; Some (t2, q1)
+       end) args t in 
+        dl = Some x -> 
+      (fix fold (l0 : list type) (dl : DList.T (fun H0 : type => sval H0) l0)
+           {struct dl} : option (Tuple.of_list eval_type l0) :=
+       match
+         dl in (DList.T _ l1) return (option (Tuple.of_list eval_type l1))
+       with
+         | DList.nil => Some tt
+         | DList.cons t0 q0 t1 q =>
+             do t2 <- eval_sval t0 t1 (l ++ l');
+             do q1 <- fold q0 q; Some (t2, q1)
+       end) args t  = Some x
+         ). 
+  clear - H. induction t.
+  simpl. auto. 
+  
+  simpl. intros. 
+  
+  simpl in H. destruct H as [Hhd Htl]. specialize (IHt Htl).
+  case_eq (eval_sval t p l). 
+  intros. rewrite H in H0.  apply Hhd in H. rewrite H. simpl. simpl in H0. 
+  invert_do H0. apply IHt in EQ.  rewrite EQ. simpl. reflexivity. 
+  intros.
+  rewrite H in H0. simpl in H0. discriminate. 
+  intros H'. invert_do H'. apply H0 in EQ. rewrite EQ. simpl. 
+  reflexivity. 
+Qed. 
+
+Lemma list_in_snoc {A} l (x y : A) : List.In x (l++[y]) -> List.In x l \/  x = y. 
+Proof. 
+  revert x y. induction l. simpl; intuition.
+  simpl. intros x y [H | H]; auto. 
+  apply IHl in H. intuition.
+Qed. 
+  
+
+Lemma nth_error_map {A B} {f : A -> B} l t  :
+  List.nth_error (List.map f (l ++ [t])) (List.length l) = Some (f t). 
+Proof. 
+  induction l. reflexivity. 
+  simpl. auto. 
+Qed. 
+
+Section protect0. 
+Import Equality. 
+Lemma cse_expr_correct_2 Phi st G env (Hg : Gamma_inv G env) t:
+  forall e1 e2, expr_equiv eval_type V Phi (Flat.R eval_type V G) t e1 e2 ->
+           forall svo e, cse_expr Phi eval_type t e2 = (e,svo) ->
+                           eval_expr Phi st t e1 = eval_expr Phi st t e. 
+Proof.
+  intros e1. destruct e1; intros e2 H; inversion H; t; simpl; intros; unfold Flat.R in *. 
+  - injection H0; intros; subst. clean. reflexivity. 
+  - injection H0; intros; subst. clean. use. reflexivity. 
+  - injection H0; intros; subst. clean. simpl. f_equal.
+    clear H b. induction args. 
+    + repeat DList.inversion.  simpl. reflexivity. 
+    +   repeat DList.inversion. simpl. apply DList.inversion_pointwise in H2. destruct H2.  f_equal. eauto.  apply IHargs. auto. 
+  -  injection H0; intros; subst. clean. reflexivity. 
+  -  injection H0; intros; subst. clean. simpl. repeat use; reflexivity. 
+  - destruct dl2. simpl in H0. 
+    dependent destruction s;  injection H0; intros; subst; clean;
+    simpl; use; reflexivity. 
+  - destruct dl2. simpl in H0. 
+    dependent destruction s;  injection H0; intros; subst; clean;
+    simpl; use; reflexivity.        
+  - destruct dl2. simpl in H0. 
+    dependent destruction s;  injection H0; intros; subst; clean;
+    simpl; use; reflexivity.      
+  - injection H0; intros; subst; clean. simpl. 
+    clear H. 
+     induction l. 
+    + repeat DList.inversion.  simpl. reflexivity. 
+    +   repeat DList.inversion. simpl. apply DList.inversion_pointwise in H3. destruct H3.  f_equal. eauto.  apply IHl. auto. 
+Qed. 
+End protect0. 
+
+Lemma Gamma_inv_cons_var G env (Hg : Gamma_inv G env) t (e : eval_type t): 
+      Gamma_inv (cons eval_type V t e (e, SVar t (Datatypes.length env)) G)
+                (add eval_type t (SVar t (Datatypes.length env)) e env). 
+Proof.
+  intros. 
+  constructor; intros. 
+  - inversion H; t. reflexivity.  use; reflexivity.  
+  - inversion H; t. simpl. unfold lift. unfold add. simpl. 
+    rewrite nth_error_map. simpl.
+    
+    apply type_cast_eq.
+    apply (Gamma_inv_2 _ _ Hg) in H1.
+    clear - H1. 
+    unfold lift, add in *. 
+
+    destruct y as [ y sv]. 
+    rewrite List.map_app. 
+    revert H1. 
+    match goal with |- context [List.map ?f _] => set (F := f) end. 
+    replace (List.length env) with (List.length (List.map F env)) by apply List.map_length.
+    generalize (List.map F env).  intros. simpl. 
+    clear F. simpl in H1.  
+    apply eval_sval_monotone ; auto.    
+    
+    
+  - unfold add in H.  apply list_in_snoc in H. 
+    destruct H. apply In_skip. eauto. 
+    t. apply In_ok. congruence. congruence. 
+Qed.         
+      
+Lemma Gamma_inv_cons_other G env (Hg : Gamma_inv G env) t (e : eval_type t) sv: 
+  eval_sval t sv (lift env) = Some e ->
+  Gamma_inv (cons eval_type V t e (e, sv) G)
+            (add eval_type t sv e env). 
+Proof. 
+  constructor. 
+  - intros. inversion H0; subst; t; subst. reflexivity.   eauto. 
+  - intros. inversion H0; subst; t; subst. 
+    simpl. unfold lift, add. rewrite List.map_app. apply eval_sval_monotone. apply H.
+    simpl. unfold lift, add. rewrite List.map_app. apply eval_sval_monotone. eapply Gamma_inv_2; eauto. 
+  - intros.
+  unfold add in H0; apply list_in_snoc in H0. 
+  destruct H0. apply In_skip. eauto. 
+  t. apply In_ok. congruence. 
+  congruence. 
+Qed. 
+
+
 Theorem cse_correct Phi st t  Delta: 
      forall (b : block Phi eval_type t)
      (b' : block Phi V t)
-     (e : Env Phi eval_type)
      (G : Gamma eval_type V),
        block_equiv eval_type V Phi t G b b' ->
-     (forall t (x : eval_type t) y, G |- x -- y -> x = fst y)  ->
-     (forall t (x : eval_type t) y, G |- x -- y -> eval_sval Phi st t (snd y) (lift e) = Some x)
+       forall e,
+       Gamma_inv G e
      ->
    eval_telescope Phi st
      (fun x : eval_type t * bool * effects Phi eval_type =>
@@ -310,67 +758,56 @@ Theorem cse_correct Phi st t  Delta:
       (let (p, e0) := k in
        let (v, g) := p in & (fst v, fst g, cse_effects Phi eval_type e0))). 
 Proof. 
-  induction 1. 
-  simpl. intros. admit. 
-  simpl. intros. 
-  case_eq (cse_expr Phi eval_type a e2). intros. 
-  destruct o. simpl. 
-  case_eq (lookup Phi eval_type a s e). intros.
-  apply H1. clear H1. 
+  induction 1.
   
-  assert (eval_expr Phi st a e0 = eval_expr Phi st a e1). 
-  admit. 
-  rewrite <- H1. 
+  * simpl; intros; repeat use.
+  simpl eval_type;
+  match goal with |- context [check ?x; _] => destruct x; [|reflexivity]  end. 
+  f_equal.   f_equal. 
+  eapply cse_effects_correct; eauto. 
   
-  forall G b b', 
-    Flat.block_equiv _ _ Phi t G  b b' -> 
-    Flat.eval_block Phi st t b Delta = Flat.eval_block Phi st t (cse_block Phi _ t b') Delta.      
-Proof.  
-  unfold eval_block. unfold cse_block. 
-  generalize (empty Phi eval_type).
-  
-  intros e b b' H. revert e.  revert b b' H. induction 1. 
-  
-  simpl. intros.  
-  subst. simpl.  
-  repeat match goal with 
-             |- context [check ?x ; _] => destruct x
-         end; try reflexivity.
-  subst. 
-  f_equal. f_equal.
-  admit.
+  * intros; simpl eval_telescope. clear H0. 
+    case_eq (cse_expr Phi eval_type a e2). 
+    destruct o. 
+    case_eq (lookup eval_type a s (e)). intros. 
+    simpl. 
+    apply H1.
 
-  simpl. 
-  case_eq (cse_expr Phi eval_type a e2). 
-  intros e o Heo env. 
-  case_eq o. simpl. intros. subst. simpl.
-  case_eq (lookup Phi eval_type a s env).  intros.
-  erewrite <- H1. 
-  reflexivity. 
-  clear H1 . 
-  clear H0. 
-  simpl. 
+    { now_show ( Gamma_inv (cons eval_type V a (eval_expr Phi st a e1) (e3, s) G) e). 
+      assert (eval_expr Phi st a e1 = e3). 
+      pose proof (lem1 Phi st e G a _ _ _ s H H2 H3).
+       
+      eauto using lemma_2. 
+      rewrite H4. 
+      apply Gamma_inv_cons. auto. subst; eauto using lem1. 
+    }
+    
+    intros. simpl. 
+    apply H1. 
+    assert (eval_expr Phi st a e0 = eval_expr Phi st a e1). 
+    pose proof (H3). eapply lem1 in H4; eauto. 
+    symmetry; eapply cse_expr_correct_2; eauto. 
+    rewrite H4. 
+    
+    
+    {
+      clear H1. clear H4.
+      assert (eval_sval a s (lift e) = Some (eval_expr Phi st a e1)). eauto using lem1. 
+      
+      apply Gamma_inv_cons_other; auto. 
+    }
+    
+    intros. 
+    apply H1.
+    { clear H1. 
+    assert (eval_expr Phi st a e1 = eval_expr Phi st a e0). 
+    eapply cse_expr_correct_2; eauto. 
+    rewrite H1 in *. generalize (eval_expr Phi st a e0). 
+    clear  H1.   clear -H2.
+    apply Gamma_inv_cons_var; auto. }
 
 
-  Lemma lemma Phi st t sv env e : lookup Phi eval_type t sv env = Some e -> 
-              eval_sval Phi st t sv (lift Phi (content _ _ env)) = Some e. 
-  Proof. 
-  Admitted.
-  
-  Lemma cse_expr_correct Phi st t env e e' e'' sv : cse_expr Phi eval_type t e = (e', Some sv) -> 
-                             eval_sval Phi st t sv env = Some e'' -> 
-                             eval_expr Phi st t e' = e''. 
-  Admitted.
-pose (h' := Heo). 
-eapply cse_expr_correct in h'.
-2 : apply lemma.  2: apply H2. 
-erewrite cse_expr_correct. 
-eapply cse_expr_correct. apply Heo.  eauto. 
-
-  intros.  simpl. erewrite <- H1.  reflexivity. 
-  admit. 
-  
-  intros. subst.  
-  simpl. erewrite <- H1. reflexivity. 
-  admit. 
-Qed. *)
+    Grab Existential Variables. 
+    apply st. 
+Qed. 
+Print Assumptions cse_correct.
